backend/Tailcallproof.v
@@ -13,7 +13,6 @@
 (** Recognition of tail calls: correctness proof *)
 
 Require Import Coqlib.
-Require Import Compopts.
 Require Import Maps.
 Require Import AST.
 Require Import Integers.
@@ -183,10 +182,9 @@ Lemma transf_instr_lookup:
   exists i',  (transf_function f).(fn_code)!pc = Some i' /\ transf_instr_spec f i i'.
 Proof.
   intros. unfold transf_function.
-  destruct (zeq (fn_stacksize f) 0). destruct (eliminate_tailcalls tt).
+  destruct (zeq (fn_stacksize f) 0).
   simpl. rewrite PTree.gmap. rewrite H. simpl. 
   exists (transf_instr f pc i); split. auto. apply transf_instr_charact; auto. 
-  exists i; split. auto. constructor.
   exists i; split. auto. constructor.
 Qed.
 
@@ -263,14 +261,14 @@ Lemma sig_preserved:
   forall f, funsig (transf_fundef f) = funsig f.
 Proof.
   destruct f; auto. simpl. unfold transf_function. 
-  destruct (zeq (fn_stacksize f) 0 && eliminate_tailcalls tt); auto. 
+  destruct (zeq (fn_stacksize f) 0); auto. 
 Qed.
 
 Lemma stacksize_preserved:
   forall f, fn_stacksize (transf_function f) = fn_stacksize f.
 Proof.
   unfold transf_function. intros. 
-  destruct (zeq (fn_stacksize f) 0 && eliminate_tailcalls tt); auto.
+  destruct (zeq (fn_stacksize f) 0); auto.
 Qed.
 
 Lemma find_function_translated:
@@ -556,7 +554,7 @@ Proof.
   assert (fn_stacksize (transf_function f) = fn_stacksize f /\
           fn_entrypoint (transf_function f) = fn_entrypoint f /\
           fn_params (transf_function f) = fn_params f).
-    unfold transf_function. destruct (zeq (fn_stacksize f) 0 && eliminate_tailcalls tt); auto. 
+    unfold transf_function. destruct (zeq (fn_stacksize f) 0); auto. 
   destruct H0 as [EQ1 [EQ2 EQ3]]. 
   left. econstructor; split.
   simpl. eapply exec_function_internal; eauto. rewrite EQ1; eauto.
